WeakOmegaCat/.dir-locals.el
@@ -2,7 +2,7 @@
   . ((eval . 
 	   (progn
 	     (make-local-variable 'coq-prog-args)
-         (setq coq-prog-name "~/coq/coqIR/coq/bin/coqtop")
+         (setq coq-prog-name "~/Prog/coq/IR/coq/bin/coqtop")
 	      (if (not (memq 'agda-input features))
                  (load (concat "~/coq/UniMath/" "emacs/agda/agda-input")))
              (if (not (member '("chimney" "╝") agda-input-user-translations))
